# **Bayesian networks** *Principles and Definitions*

# The focus today . . .

#### Probability theory

- Joint probability
- Marginal probability
- Conditional probability
- Chain rule
- Bayes' rule

#### Bayesian networks

- Definition
- Conditional independence

# **Intelligent patient monitoring at home**



# Why Bayesian networks?

Probabilistic graphical models, such as Bayesian networks, are now the most popular uncertainty formalisms because:

- Handle noise, missing information and probabilistic relations
- Learn from data and can incorporate domain knowledge
- Offer flexible reasoning
- Have compact graphical representation (interface)
- Founded principles: probability theory
- Engineering principles: knowledge acquisition, machine learning and statistics

# **General notation**

- Stochastic (= statistical = random) variable: upper-case letter, e.g. X, or upper-case string, e.g. FEVER
- Values: variables can take on values, e.g. X = x, FEVER = yes
- Binary variables: take one of two values, e.g. X = true and X = false
- Discrete variables: take only one of a finite set of possible values, e.g. TEMP ∈ {*low, medium, high*}
- Continuous variables: take any value in some interval or intervals of real numbers  $\mathcal{R}$ , e.g.  $\text{TEMP} \in [-50, 50]$

#### **Abbreviated notation**

- Binary variables: X = true as x, and X = false as  $\neg x$
- Non-binary variables: X = x as x or CITY = tokyo as tokyo
- Sets of variables: analogous to variables
   Example:

 $X_n = x_n$ 

$$X_{1} = x_{1}$$

$$X_{2} = x_{2}$$

$$X = (X_{1}, X_{2}, \dots, X_{n})$$

$$\therefore \qquad \Longrightarrow \qquad x = (x_{1}, x_{2}, \dots, x_{n})$$

$$X = x$$

Lecture2: Bayesian networks - p.6

## **Abreviated notation (cont.)**

- Conjunctions:  $(X = x) \land (Y = y)$  as (X = x, Y = y)
- Templates: (X, Y) means (X = x, Y = y), for any value x, y, i.e. the choice of the values x and y does not really matter
- Examples:
  - $P(X = x, Y = y) \Leftrightarrow P(X = x \land Y = y)$
  - $P(X,Y) \Leftrightarrow P(X=x,Y=y)$ , for any value x,y
  - $P(X \mid Y) \Leftrightarrow P(X = x \mid Y = y)$ , for any value x, y

• 
$$\sum_{X} P(X) = P(x) + P(\neg x)$$
, where X is binary

# **Probability theory**

- Probability distribution P: attaches a number in (closed) interval [0, 1] to Boolean expressions
- Boolean algebra B (for two variables RAIN and HAPPY):

```
\top (true),
rain, \negrain,
happy, \neghappy,
rain \land happy,..., rain \land happy \land \neghappy,...,
\negrain \land happy,..., rain \lor happy,
\bot (false)
```

such that:

•  $\perp \leq rain, rain \leq (rain \lor happy), \dots$  (in general  $\perp \leq x$  for each Boolean expression  $x \in \mathbb{B}$ );

•  $x \leq \top$  for each Boolean expression  $x \in \mathbb{B}$ 

# **Probability distribution**

- A probability distribution *P* is defined as a function  $P: \mathbb{B} \to [0, 1]$ , such that:
  - $P(\perp) = 0$
  - $P(\top) = 1$
  - $P(x \lor y) = P(x) + P(y)$ , if  $x \land y = \bot$  with  $x, y \in \mathbb{B}$

#### Examples:

- $P(rain \lor happy) = P(rain) + P(happy)$ , as rain  $\land happy = \bot$  (why? Because I define it that way)
- $P(rain \land happy) = P(\bot) = 0$
- $P(\neg rain \lor rain) = P(\neg rain) + P(rain) = P(\top) = 1 \Rightarrow$  $P(\neg rain) = 1 - P(rain)$
- $0 \le P(rain) \le 1$

# **Probability distribution (cont.)**

- Boolean algebras  $\Leftrightarrow$  sets:
  - $\bullet \ \top \Leftrightarrow \Omega \qquad \qquad \bullet \ (x \lor y) \Leftrightarrow (X \cup Y)$
  - $\bot \Leftrightarrow \varnothing$   $(x \land y) \Leftrightarrow (X \cap Y)$
  - $x \Leftrightarrow X$
  - $\neg x \Leftrightarrow \bar{X}$

•  $x \le (x \lor y) \Leftrightarrow X \subseteq (X \cup Y)$ 

with  $\Leftrightarrow$  1-1 correspondence, e.g.

$$P(\overline{\text{Rain}}) = 1 - P(\text{Rain})$$

# Joint probability distribution

Let X and Y be random variables with domains

$$dom(X) = \{x_1, x_2, \dots, x_n\}$$
 and  $dom(Y) = \{y_1, y_2, \dots, y_m\}.$ 

The product set

$$dom(X) \times dom(Y) = \{x_1, x_2, \dots, x_n\} \times \{y_1, y_2, \dots, y_m\}$$

is made into a probability space by defining

$$P(X = x_i \land Y = y_j) = P(x_i, y_j)$$

where P is a joint probability function of X and Y.

## **Marginalisation**

Suppose the joint probability distribution of two variables X and Y is given; then

$$P(x) = P(X = x) = P(x \land \top)$$
  
=  $P(x \land (y \lor \neg y))$   
=  $P((x \land y) \lor (x \land \neg y))$   
=  $P(x \land y) + P(x \land \neg y)$ 

since  $P(a \lor b) = P(a) + P(b)$ , if  $a \land b = \bot$ 

$$\implies P(x) = \sum_{Y} P(x, Y)$$

also known as marginal probability function of X.

# Example

• Assume that  $X_1$ ,  $X_2$ ,  $X_3$  and  $X_4$  are binary variables. Then  $P(X1, X_2, X_3, X_4)$ :

$P(x_1, x_2, x_3, x_4)$	=	0.1	$P(x_1, \neg x_2, \neg x_3, x_4)$	=	0.015
$P(x_1, \neg x_2, x_3, x_4)$	=	0.04	$P(x_1,\neg x_2,x_3,\neg x_4)$	=	0.1
$P(x_1, x_2, \neg x_3, x_4)$	=	0.03	$P(x_1, x_2, \neg x_3, \neg x_4)$	=	0.004
$P(x_1, x_2, x_3, \neg x_4)$	=	0.1	$P(\neg x_1, \neg x_2, \neg x_3, x_4)$	=	0.005
$P(\neg x_1, x_2, x_3, x_4)$	=	0.0	$P(\neg x_1, \neg x_2, x_3, \neg x_4)$	=	0.01
$P(\neg x_1, \neg x_2, x_3, x_4)$	=	0.2	$P(\neg x_1, x_2, \neg x_3, \neg x_4)$	=	0.01
$P(\neg x_1, x_2, \neg x_3, x_4)$	=	0.08	$P(x_1, \neg x_2, \neg x_3, \neg x_4)$	=	0.006
$P(\neg x_1, x_2, x_3, \neg x_4)$	=	0.1	$P(\neg x_1, \neg x_2, \neg x_3, \neg x_4)$	=	0.2

- $\sum_{X_1, X_2, X_3, X_4} P(X_1, X_2, X_3, X_4) = 1$
- Marginalisation:

$$P(x_2, \neg x_3) = ?$$

Lecture2: Bayesian networks - p.13

# **Conditional probability**

- $P(X \mid Y)$ : Chance that X will occur knowing that Y has occured
- Definition:

$$P(X \mid Y) = \frac{P(X \cap Y)}{P(Y)}$$

$$\nearrow$$
normalize, so
that uncertainty in Y
is removed

# **Example:** *flu* and *fever*

- $P(flu \wedge fever)$ : chance of flu and fever at the same time
- $P(flu \mid fever)$ : chance of flu knowing that the person already has *fever* (conditional probability)
- Definition:

 $P(\mathbf{flu} \mid \mathbf{fever}) = \frac{P(\mathbf{flu} \land \mathbf{fever})}{P(\mathbf{fever})}$ adjust  $P(flu \wedge fever)$ , so that uncertainty in 'fever' is removed

**P** Recall:  $P(Flu \cap Fever)$  is different notation, with same meaning as  $P(flu \wedge fever)$ 

## **Reversal of chances**

•  $P(flu \mid fever)$  is usually unknown:



### **Bayes' rule - Example**

Bayes' rule – reversal of chances:

 $\begin{array}{ll} P(e \mid h) & P(\textit{fever} \mid \textit{flu}) = 0.9\\ P(h) & P(\textit{flu}) = 0.05\\ P(e) & P(\textit{fever}) = 0.09 \end{array}$ 

$$P(\textit{flu} | \textit{fever}) = \frac{P(\textit{fever} | \textit{flu})P(\textit{flu})}{P(\textit{fever})}$$
$$= 0.9 \cdot 0.05/0.09 = 0.5$$

Definition of Bayes' rule (the 'chance reverter'):

$$P(h \mid e) = \frac{P(e \mid h)P(h)}{P(e)}$$

## **Chain rule (derivation)**

Definition of conditional probability:

$$P(X_1 \mid X_2, \dots, X_n) = \frac{P(X_1, X_2, \dots, X_n)}{P(X_2, \dots, X_n)}$$

$$\Rightarrow P(X_1, X_2, \dots, X_n) = P(X_1 \mid X_2, \dots, X_n) P(X_2, \dots, X_n)$$

Furthermore,

$$P(X_2, \dots, X_n) = P(X_2 \mid X_3, \dots, X_n) P(X_3, \dots, X_n)$$
  

$$\vdots \vdots \vdots$$
  

$$P(X_{n-1}, X_n) = P(X_{n-1} \mid X_n) P(X_n)$$
  

$$P(X_n) = P(X_n)$$

# **Chain rule (definition)**

$$P(X_1, X_2, \dots, X_n) = P(X_1 \mid X_2, \dots, X_n) \cdot P(X_2 \mid X_3, \dots, X_n) \cdot P(X_3 \mid X_4, \dots, X_n) \cdot \vdots$$

$$P(X_{n-1} \mid X_n) \cdot P(X_n)$$

$$= \prod_{i=1}^{n-1} P(X_i \mid X_{i+1}, \dots, X_n) P(X_n)$$

# **Definition Bayesian network (BN)**

A Bayesian network  $\mathcal{B}$  is a pair  $\mathcal{B} = (G, P)$ , where:

- G = (V(G), A(G)) is an acyclic directed graph, with
  V(G) = {v<sub>1</sub>, v<sub>2</sub>,..., v<sub>n</sub>}, a set of vertices (nodes)
  A(G) ⊆ V(G) × V(G) a set of arcs
- $P: \wp(V(G)) \to [0,1]$  is a joint probability distribution, such that

$$P(V(G)) = \prod_{i=1}^{n} P(v_i \mid \pi_G(v_i))$$

where  $\pi_G(v_i)$  denotes the set of immediate ancestors (parents) of vertex  $v_i$  in G

• Notational convenience:  $v_i \approx X_i$ 

# **Example of a Bayesian network**



Bayesian network  $\mathcal{B} = (G, P)$ , where G = (V(G), A(G)), with

- **Set of vertices:**  $V(G) = \{X_1, X_2, X_3\}$
- **Set of arcs:**  $A(G) = \{(X_1, X_2), (X_1, X_3)\}$
- Joint probability distribution:

$$P(X_1, X_2, X_3) = P(X_1) \cdot P(X_2 \mid X_1) \cdot P(X_3 \mid X_1)$$

## **Example (cont.)**

$$P(X_1, X_2, X_3) = P(X_1) \cdot P(X_2 \mid X_1) \cdot P(X_3 \mid X_1)$$

with for example:

$$P(x_1) = 0.7$$

$$P(\neg x_1) = 0.3 = 1 - P(x_1)$$

$$P(x_2 \mid x_1) = 0.6$$

$$P(x_2 \mid x_1) = 0.4$$

$$P(\neg x_2 \mid x_1) = 0.4$$

$$P(\neg x_3 \mid x_1) = 0.9$$

$$P(x_2 \mid \neg x_1) = 0.1$$

$$P(x_3 \mid \neg x_1) = 0.8$$

$$P(\neg x_2 \mid \neg x_1) = 0.9$$

$$P(\neg x_3 \mid \neg x_1) = 0.2$$

# **Conditional independence relation**

Let X, Y, Z be sets of variables, such that  $X, Y, Z \subseteq V(G)$ , then X is called conditionally independent of Y given Z, denoted as

 $X \perp\!\!\!\perp_P Y \mid Z$ 

if and only if

$$P(X \mid Y, Z) = P(X \mid Z)$$

**Example:** Representation of  $X_2 \perp P X_3 \mid X_1$  in a directed graph



# **Chain rule - digraph**



Factorisation (1):

 $P(X_1, X_2, X_3) = P(X_1 \mid X_2, X_3) P(X_2 \mid X_3) P(X_3)$ 

Other factorisation (2):

 $P(X_1, X_2, X_3) = P(X_2 \mid X_1, X_3) P(X_1 \mid X_3) P(X_3)$ 

 $\Rightarrow$  different *factorisations* possible

#### **Does the chain rule help?**



 $P(X_1, X_2, X_3) = P(X_1 \mid X_2, X_3) P(X_2 \mid X_3) P(X_3)$ 

i.e. we need:

$$\begin{array}{cccccccccccc}
P(x_1 \mid x_2, x_3) & P(x_1 \mid x_2, \neg x_3) \\
P(\neg x_1 \mid x_2, x_3) & P(\neg x_1 \mid x_2, \neg x_3) \\
P(x_1 \mid \neg x_2, x_3) & P(x_1 \mid \neg x_2, \neg x_3) \\
P(\neg x_1 \mid \neg x_2, x_3) & P(\neg x_1 \mid \neg x_2, \neg x_3) \\
\vdots & \vdots & \vdots & \vdots \\
\end{array}$$

## **Does the chain rule help?**

$$P(x_2 \mid x_3) \qquad P(x_3)$$

$$P(\neg x_2 \mid x_3) \qquad P(\neg x_3)$$

$$P(x_2 \mid \neg x_3)$$

$$P(\neg x_2 \mid \neg x_3)$$

#### So, 14 probabilities; however $P(x_1 | X_2, X_3) = 1 - P(\neg x_1 | X_2, X_3),$ $P(x_2 | X_3) = 1 - P(\neg x_2 | X_3),$ and $P(x_3) = 1 - P(\neg x_3)$

 $\Rightarrow$  7 probabilities required

How many did we have originally for  $P(X_1, X_2, X_3)$ ?

#### **Does the chain rule help?**

$$P(x_1, x_2, x_3) \qquad P(x_1, x_2, \neg x_3) \\ P(\neg x_1, x_2, x_3) \qquad P(\neg x_1, x_2, \neg x_3) \\ P(x_1, \neg x_2, x_3) \qquad P(x_1, \neg x_2, \neg x_3) \\ P(\neg x_1, \neg x_2, x_3) \qquad P(\neg x_1, \neg x_2, \neg x_3) \\ P(\neg x_1, \neg x_2, x_3) \qquad P(\neg x_1, \neg x_2, \neg x_3) \\ P(\neg x_1, \neg x_2, x_3) \qquad P(\neg x_1, \neg x_2, \neg x_3) \\ P(\neg x_1, \neg x_2, x_3) \qquad P(\neg x_1, \neg x_2, \neg x_3) \\ P(\neg x_1, \neg x_2, x_3) \qquad P(\neg x_1, \neg x_2, \neg x_3) \\ P(\neg x_1, \neg x_2, x_3) \qquad P(\neg x_1, \neg x_2, \neg x_3) \\ P(\neg x_1, \neg x_2, x_3) \qquad P(\neg x_1, \neg x_2, \neg x_3) \\ P(\neg x_1, \neg x_2, x_3) \qquad P(\neg x_1, \neg x_2, \neg x_3) \\ P(\neg x_1, \neg x_2, x_3) \qquad P(\neg x_1, \neg x_2, \neg x_3) \\ P(\neg x_1, \neg x_2, x_3) \qquad P(\neg x_1, \neg x_2, \neg x_3) \\ P(\neg x_1, \neg x_2, x_3) \qquad P(\neg x_1, \neg x_2, \neg x_3) \\ P(\neg x_1, \neg x_2, \neg x_3) \qquad P(\neg x_1, \neg x_2, \neg x_3) \\ P(\neg x_1, \neg x_2, \neg x_3) \qquad P(\neg x_1, \neg x_2, \neg x_3) \\ P(\neg x_1, \neg x_2, \neg x_3) \qquad P(\neg x_1, \neg x_2, \neg x_3) \\ P(\neg x_1, \neg x_2, \neg x_3) \qquad P(\neg x_1, \neg x_2, \neg x_3) \\ P(\neg x_1, \neg x_2, \neg x_3) \qquad P(\neg x_1, \neg x_2, \neg x_3) \\ P(\neg x_1, \neg x_2, \neg x_3) \qquad P(\neg x_1, \neg x_2, \neg x_3) \\ P(\neg x_1, \neg x_2, \neg x_3) \qquad P(\neg x_1, \neg x_2, \neg x_3) \\ P(\neg x_1, \neg x_2, \neg x_3) \qquad P(\neg x_1, \neg x_2, \neg x_3) \\ P(\neg x_1, \neg x_2, \neg x_3) \qquad P(\neg x_1, \neg x_2, \neg x_3) \\ P(\neg x_1, \neg x_2, \neg x_3) \qquad P(\neg x_1, \neg x_2, \neg x_3) \\ P(\neg x_1, \neg x_2, \neg x_3) \qquad P(\neg x_1, \neg x_2, \neg x_3) \\ P(\neg x_1, \neg x_2, \neg x_3) \qquad P(\neg x_1, \neg x_2, \neg x_3) \\ P(\neg x_1, \neg x_2, \neg x_3) \qquad P(\neg x_1, \neg x_2, \neg x_3) \\ P(\neg x_1, \neg x_2, \neg x_3) \qquad P(\neg x_1, \neg x_2, \neg x_3) \\ P(\neg x_1, \neg x_2, \neg x_3) \qquad P(\neg x_1, \neg x_2, \neg x_3) \\ P(\neg x_1, \neg x_2, \neg x_3) \qquad P(\neg x_1, \neg x_2, \neg x_3) \\ P(\neg x_1, \neg x_2, \neg x_3) \qquad P(\neg x_1, \neg x_2, \neg x_3) \\ P(\neg x_1, \neg x_2, \neg x_3) \qquad P(\neg x_1, \neg x_2, \neg x_3) \\ P(\neg x_1, \neg x_2, \neg x_3) \qquad P(\neg x_1, \neg x_2, \neg x_3) \\ P(\neg x_1, \neg x_2, \neg x_3) \qquad P(\neg x_1, \neg x_2, \neg x_3) \\ P(\neg x_1, \neg x_2, \neg x_3) \qquad P(\neg x_1, \neg x_2, \neg x_3) \\ P(\neg x_1, \neg x_2, \neg x_3) \qquad P(\neg x_1, \neg x_2, \neg x_3) \\ P(\neg x_1, \neg x_$$

8 required? No, because  $\sum_{X_1,X_2,X_3} P(X_1,X_2,X_3) = 1$ Hence, e.g.

$$P(x_1, x_2, x_3) = 1 - \sum_{X_2, X_3} P(\neg x_1, X_2, X_3)$$
$$- \sum_{X_3} P(x_1, \neg x_2, X_3) - P(x_1, x_2, \neg x_3)$$

## Let's use stochastic independence



$$P(X_1, X_2, X_3) = P(X_2 \mid X_1, X_3) P(X_3 \mid X_1) P(X_1)$$

Now assume that  $X_2$  and  $X_3$  are conditionally independent given  $X_1$ :

$$P(X_2 \mid X_1, X_3) = P(X_2 \mid X_1)$$

and

$$P(X_3 \mid X_1, X_2) = P(X_3 \mid X_1)$$

# **Stochastic independence: does it help?**



 $P(X_2 \mid X_1, X_3) = P(X_2 \mid X_1)$ 

#### $P(X_1, X_2, X_3) = P(X_2 \mid X_1, X_3) P(X_3 \mid X_1) P(X_1)$ = $P(X_2 \mid X_1) P(X_3 \mid X_1) P(X_1)$

Only 5 = 2 + 2 + 1 probabilities required instead of 7

#### **Probabilistic inference**



Given:

Then:  $P(x_4) = P(x_4, x_3) + P(x_4, \neg x_3)$ (marginalisation)  $= P(x_4 \mid x_3)P(x_3) + P(x_4 \mid \neg x_3)P(\neg x_3)$ (conditioning)  $= \sum_{X_3} P(x_4 \mid X_3)P(X_3)$ 

## **Probabilistic inference**



$$P(x_4 | x_3) = 0.4$$

$$P(x_4 | \neg x_3) = 0.1$$

$$P(x_3 | x_1, x_2) = 0.3$$

$$P(x_3 | \neg x_1, x_2) = 0.5$$

$$P(x_3 | x_1, \neg x_2) = 0.7$$

$$P(x_3 | \neg x_1, \neg x_2) = 0.9$$

$$P(x_1) = 0.6$$

$$P(x_2) = 0.2$$

 $P(X_3) = ? \iff Compute P(x_3) \text{ and } P(\neg x_3)$ 

### **Probabilistic inference**



$$P(x_3) = \sum_{X_1, X_2} P(x_3, X_1, X_2)$$
  
=  $\sum_{X_1, X_2} P(x_3 \mid X_1, X_2) P(X_1, X_2)$   
=  $\sum_{X_1, X_2} P(x_3 \mid X_1, X_2) P(X_1) P(X_2) = 0.7$ 

 $\Rightarrow P(x_4) = \sum_{X_3} P(x_4 \mid X_3) P(X_3) = 0.4 \cdot 0.7 + 0.1 \cdot 0.3 = 0.31$ 

# **Back to the mobile application**

Prediction of COPD (lung disease) exacerbations



Expert opinion based Bayesian network with prior probabilities shown (top probability is Normal state). A = activity, C = cough, D = dyspnea, E = exacerbation, F = FEV<sub>1</sub>, I = infection, LF = lung function, M = malaise, S = SpO<sub>2</sub>, SC = sputum colour, SV = sputum volume, T = temperature and W = Wheeze.

# **Popular applications of BNs**

- Medical diagnosis and therapy selection: BNs are now the most popular paradigm for medical intelligent systems
  - Mobile healthcare applications by MBSD-Radboud University
    - COPD monitoring (www.youtube.com/watch?v=zfqW8rX00pM)
    - Pregnancy monitoring (www.youtube.com/watch?v=Ize-ydS1UiU)
- Software/Hardware troubleshooting: Microsoft, Boeing, HP
- Biological modelling: gene expressions
- Art: orchestral music accompaniment

xavier.informatics.indiana.edu/~craphael/music\_plus\_one/

#### and more . . . see, e.g.,

"Bayesian Networks: A Practical Guide to Applications" Olivier Pourret (Ed.), Patrick Naïm and Bruce Marcot, Wiley, March 2008

# **Bayesian networks software**

- Some software companies in this area:
  - Hugin (Denmark): www.hugin.dk
  - Norsys (USA): www.norsys.com
  - Scheme Knowledge Industries (USA): www.kic.com
  - Bayesia (France): www.bayesia.com
- Some public domain software:
  - JavaBayes: www.cs.cmu.edu/~javabayes
  - BayesBuilder: www.snn.ru.nl/nijmegen
  - **bnlearn package in R**: www.bnlearn.com
  - Samlam: reasoning.cs.ucla.edu/samiam
  - Matlab BNT Toolbox: code.google.com/p/bnt
  - and many more at

www.cs.ubc.ca/~murphyk/Software/bnsoft.html